lean-fx-2/LeanFX2/Algo/Soundness.lean
@@ -420,6 +420,8 @@ theorem Term.headStep?_sound
   | interval1 => nomatch firedEq
   | pathLam _ _ _ _ => nomatch firedEq
   | glueIntro _ _ _ _ => nomatch firedEq
+  | transp _ _ _ _ _ _ _ _ => nomatch firedEq
+  | hcomp _ _ => nomatch firedEq
   | universeCode _ _ _ _ => nomatch firedEq
   | cumulUp _ _ _ _ _ _ => nomatch firedEq
   | equivReflId _ => nomatch firedEq
@@ -488,7 +490,7 @@ theorem Term.headStep?_sound
     | .eitherInl | .eitherInr | .eitherMatch
     | .refl | .idJ | .modIntro | .modElim | .subsume
     | .interval0 | .interval1 | .pathLam | .pathApp
-    | .glueIntro | .glueElim
+    | .glueIntro | .glueElim | .transp | .hcomp
     | .universeCode | .cumulUp
     | .equivReflId | .funextRefl | .equivReflIdAtId | .funextReflAtId
     | .equivIntroHet | .uaIntroHet | .funextIntroHet
@@ -518,7 +520,7 @@ theorem Term.headStep?_sound
     | .eitherInl | .eitherInr | .eitherMatch
     | .refl | .idJ | .modIntro | .modElim | .subsume
     | .interval0 | .interval1 | .pathLam | .pathApp
-    | .glueIntro | .glueElim
+    | .glueIntro | .glueElim | .transp | .hcomp
     | .universeCode | .cumulUp
     | .equivReflId | .funextRefl | .equivReflIdAtId | .funextReflAtId
     | .equivIntroHet | .uaIntroHet | .funextIntroHet
@@ -547,7 +549,7 @@ theorem Term.headStep?_sound
     | .eitherInl | .eitherInr | .eitherMatch
     | .refl | .idJ | .modIntro | .modElim | .subsume
     | .interval0 | .interval1 | .pathLam | .pathApp
-    | .glueIntro | .glueElim
+    | .glueIntro | .glueElim | .transp | .hcomp
     | .universeCode | .cumulUp
     | .equivReflId | .funextRefl | .equivReflIdAtId | .funextReflAtId
     | .equivIntroHet | .uaIntroHet | .funextIntroHet
@@ -576,7 +578,7 @@ theorem Term.headStep?_sound
     | .eitherInl | .eitherInr | .eitherMatch
     | .refl | .idJ | .modIntro | .modElim | .subsume
     | .interval0 | .interval1 | .pathLam | .pathApp
-    | .glueIntro | .glueElim
+    | .glueIntro | .glueElim | .transp | .hcomp
     | .universeCode | .cumulUp
     | .equivReflId | .funextRefl | .equivReflIdAtId | .funextReflAtId
     | .equivIntroHet | .uaIntroHet | .funextIntroHet
@@ -605,7 +607,7 @@ theorem Term.headStep?_sound
     | .eitherInl | .eitherInr | .eitherMatch
     | .refl | .idJ | .modIntro | .modElim | .subsume
     | .interval0 | .interval1 | .pathLam | .pathApp
-    | .glueIntro | .glueElim
+    | .glueIntro | .glueElim | .transp | .hcomp
     | .universeCode | .cumulUp
     | .equivReflId | .funextRefl | .equivReflIdAtId | .funextReflAtId
     | .equivIntroHet | .uaIntroHet | .funextIntroHet
